Checkpoint progress: - Factor copying the file to the shadow from creating and deleting the shadow. Perhaps in the future generalize this approach to make any set of operations on the shadow atomic. - Copy file attributes too.  We could also go with not copying attributes, but then we must weaken the atomic_cp spec. - Finished proof of atomic_cp_ok, assuming the following todo items are true: a few dirtree lemmas and one length lemma in file_copy

src/App.v
@@ -25,15 +25,222 @@ Set Implicit Arguments.
  * Atomic copy: create a copy of file [src_fn] in the root directory [the_dnum],
  * with the new file name [dst_fn].
  *
- * For now, this works for a single-block file, since there's no
- * byte-level file read yet.
- *
-        let^ (mscs, attr) <- FS.file_get_attr fsxp src_inum mscs;
-
  *)
 
+(* Some lemmas that should be moved to DirTree, once they are proven *)
+
+Lemma dirtree_update_add_dents: forall name elem' elem dents,
+       map (DIRTREE.update_subtree_helper (fun _ : DIRTREE.dirtree => elem') name)
+           (DIRTREE.add_to_list name elem dents) = DIRTREE.add_to_list name elem' dents.
+Proof.
+  intros.
+Admitted.
+
+Lemma dirtree_update_update_dents: forall name elem' elem tree_elem,
+    (map (DIRTREE.update_subtree_helper (fun _ : DIRTREE.dirtree => elem') name)
+         (map  (DIRTREE.update_subtree_helper (fun _ : DIRTREE.dirtree => elem) name) tree_elem))
+    =  (map (DIRTREE.update_subtree_helper (fun _ : DIRTREE.dirtree => elem') name) tree_elem).
+Proof.
+  intros.
+Admitted.
+
+
+Lemma dirtree_delete_add_dents: forall temp_fn elem tree_elem,
+  DIRTREE.delete_from_list temp_fn (DIRTREE.add_to_list temp_fn elem tree_elem)
+  = tree_elem.
+Proof.
+  intros.
+Admitted.
+
+Lemma dirtree_find_add_dents': forall temp_fn elem tree_elem,
+  fold_right
+     (DIRTREE.find_subtree_helper (fun tree : DIRTREE.dirtree => Some tree)
+        temp_fn) None
+     (DIRTREE.add_to_list temp_fn elem tree_elem) = Some elem.
+Proof.
+  intros.
+Admitted.
+  
+Lemma dirtree_find_add_dents: forall temp_fn elem tree_elem,
+  DIRTREE.find_dirlist temp_fn (DIRTREE.add_to_list temp_fn elem tree_elem)
+  = Some elem.
+Proof.
+  induction tree_elem.
+  intros; subst; simpl.
+  destruct (string_dec temp_fn temp_fn); auto.
+  congruence.
+  - destruct a.
+    destruct (string_dec temp_fn s); subst; simpl.
+    destruct (string_dec s s); simpl.
+    destruct (string_dec s s); auto. exfalso. auto.
+    exfalso; auto.
+    destruct (string_dec s temp_fn).
+    exfalso. auto.
+    simpl.
+    destruct (string_dec s temp_fn).
+    exfalso. auto.
+    rewrite IHtree_elem; reflexivity.
+Qed.
+    
+
+Lemma dirtree_add_dents_ne : forall name name' elem tree_elem,
+   name <> name' ->
+    fold_right
+      (DIRTREE.find_subtree_helper (fun tree : DIRTREE.dirtree => Some tree) name) None
+      (DIRTREE.add_to_list name' elem tree_elem) =
+    fold_right
+      (DIRTREE.find_subtree_helper (fun tree : DIRTREE.dirtree => Some tree) name) None
+      tree_elem.
+Proof.
+    intros.
+Admitted.
+
+
+Lemma dirtree_find_update_dents: forall dnum temp_fn elem tree_elem,
+  DIRTREE.find_subtree [temp_fn]
+     (DIRTREE.TreeDir dnum
+     (map (DIRTREE.update_subtree_helper
+             (fun _ : DIRTREE.dirtree => elem) temp_fn) tree_elem)) = Some elem.
+Proof.
+  unfold DIRTREE.find_subtree.
+  intros.
+Admitted.
+
+Lemma dirtree_prune_add_dents: forall inum dents temp_fn elem tree_elem,
+  dents = (DIRTREE.add_to_list temp_fn elem tree_elem)
+   -> DIRTREE.tree_prune inum dents [] temp_fn
+        (DIRTREE.TreeDir inum dents) = DIRTREE.TreeDir inum tree_elem.
+Proof.
+  intros.
+  unfold DIRTREE.tree_prune.
+  unfold DIRTREE.update_subtree.
+  unfold DIRTREE.delete_from_dir.
+  rewrite H.
+  rewrite dirtree_delete_add_dents.
+  auto.
+Qed.
+
+Lemma dirtree_graft_add_dents_eq: forall dnum tree_elem temp_fn elem,
+  DIRTREE.tree_graft dnum tree_elem [] temp_fn elem (DIRTREE.TreeDir dnum tree_elem) =
+  DIRTREE.TreeDir dnum (DIRTREE.add_to_list temp_fn elem tree_elem).
+Proof.
+  intros.
+  unfold DIRTREE.tree_graft.
+  unfold DIRTREE.update_subtree.
+  unfold DIRTREE.add_to_dir.
+  reflexivity.
+Qed.  
+     
 Parameter the_dnum : addr.
 Definition temp_fn := ".temp"%string.
+
+(* copy an existing src into an existing, empty dst. *)
+Definition file_copy T fsxp src_inum dst_inum mscs rx : prog T :=
+        (* XXX no need to do get_sz and get_attr, because get_attr has the size? *)
+  let^ (mscs, sz) <- FS.file_get_sz fsxp src_inum mscs;
+  let^ (mscs, sattr) <- FS.file_get_attr fsxp src_inum mscs;
+  let^ (mscs, b) <- FS.read_bytes fsxp src_inum 0 (# sz) mscs;
+  let^ (mscs, ok) <- FS.append fsxp dst_inum 0 (BYTEFILE.buf_data b) mscs;  (* first append *)
+  let^ (mscs, ok1) <- FS.file_set_attr fsxp dst_inum sattr mscs;   (* then set_attr *)
+  rx ^(mscs, ok && ok1).
+
+
+Theorem file_copy_ok : forall fsxp src_fn src_inum dst_fn dst_inum mscs,
+  {< m Fm Ftop tree tree_elem attr bytes,
+  PRE  LOG.rep (FSXPLog fsxp) (sb_rep fsxp) (NoTransaction m) mscs * 
+        [[ (Fm * DIRTREE.rep fsxp Ftop tree)%pred (list2mem m) ]] *
+        [[ tree = DIRTREE.TreeDir the_dnum tree_elem ]] *
+        [[ src_fn <> dst_fn ]] *
+        [[ DIRTREE.find_subtree [src_fn] tree = Some (DIRTREE.TreeFile src_inum bytes attr) ]] *
+        [[ DIRTREE.find_subtree [dst_fn] tree = Some (DIRTREE.TreeFile dst_inum [] BYTEFILE.attr0) ]]
+  POST RET:^(mscs, r)
+    exists m' tree',
+      LOG.rep (FSXPLog fsxp) (sb_rep fsxp) (NoTransaction m') mscs *
+      [[ (Fm * DIRTREE.rep fsxp Ftop tree')%pred (list2mem m') ]] *
+      (([[r = false ]] * [[ tree' = tree]]) \/
+       ([[r = false ]] *
+        exists bytes' attr',
+          [[ tree' = DIRTREE.update_subtree [dst_fn]
+                                            (DIRTREE.TreeFile dst_inum bytes' attr') tree ]]) \/
+       ([[r = true ]] *
+        [[ tree' = DIRTREE.update_subtree [dst_fn]
+                                          (DIRTREE.TreeFile dst_inum bytes attr) tree ]]))
+  CRASH any
+  >} file_copy fsxp src_inum dst_inum mscs.
+Proof.
+  unfold file_copy; intros.
+  step.
+  instantiate (pathname := [src_fn]).
+  eauto.
+  step.
+  instantiate (pathname := [src_fn]).
+  eauto.
+  step.
+  instantiate (pathname := [src_fn]).
+  eauto.
+
+ 
+  eapply pimpl_ok2. eauto with prog. cancel.  (* append step instantiates incorrectly *)
+  instantiate (pathname := [dst_fn]).
+  instantiate (bytes0 := []).
+  instantiate (attr0 := BYTEFILE.attr0).
+  eauto.
+
+  instantiate (Fi := emp).
+  constructor.
+  eauto.
+
+  step. (* set_attr *)
+  
+  instantiate (pathname := [dst_fn]).
+  instantiate (bytes0 := []).
+  instantiate (attr0 := BYTEFILE.attr0).
+  eauto.
+
+  step.  (* return *)
+  
+  subst. pimpl_crash. cancel. apply pimpl_any.
+
+  instantiate (pathname0 := [dst_fn]).
+  instantiate (bytes1 := bytes').
+  instantiate (attr1 := BYTEFILE.attr0).
+  eauto.
+
+  rewrite H18.
+  rewrite dirtree_find_update_dents; auto.
+  
+  step.   (* set_attr is ok *)
+  
+
+  eapply pimpl_or_r. right.
+  eapply pimpl_or_r. right.
+  cancel.
+
+  assert (bytes = bytes').
+  eapply star_emp_pimpl in H17.
+  apply list2nmem_array_eq in H17.
+  rewrite Nat.min_r in H12.
+  apply arrayN_list2nmem in H9.
+  unfold skipn in H9.
+  rewrite Array.firstn_oob in H9.
+  rewrite H9 in H17.
+  eauto.
+  admit.  (* H12 *)
+  admit.  (* Bytes.byte *)
+  omega.
+  rewrite <- H.
+
+  rewrite dirtree_update_update_dents; auto.
+  
+  subst. pimpl_crash. cancel. apply pimpl_any.
+  subst. pimpl_crash. cancel. apply pimpl_any.
+  subst. pimpl_crash. cancel. apply pimpl_any.
+  subst. pimpl_crash. cancel. apply pimpl_any.
+  subst. pimpl_crash. cancel. apply pimpl_any.
+Admitted.
+
+
+Hint Extern 1 ({{_}} progseq (file_copy _ _ _ _) _) => apply file_copy_ok : prog.
 
 Definition atomic_cp T fsxp src_fn dst_fn mscs rx : prog T :=
   let^ (mscs, maybe_src_inum) <- FS.lookup fsxp the_dnum [src_fn] mscs;
@@ -47,9 +254,7 @@ Definition atomic_cp T fsxp src_fn dst_fn mscs rx : prog T :=
       match maybe_dst_inum with
       | None => rx ^(mscs, false)
       | Some dst_inum =>
-        let^ (mscs, sz) <- FS.file_get_sz fsxp src_inum mscs;
-        let^ (mscs, b) <- FS.read_bytes fsxp src_inum 0 (# sz) mscs;
-        let^ (mscs, ok) <- FS.append fsxp dst_inum 0 (BYTEFILE.buf_data b) mscs;
+        let^ (mscs, ok) <- file_copy fsxp src_inum dst_inum mscs;
         match ok with
         | false =>
           let^ (mscs, ok) <- FS.delete fsxp the_dnum temp_fn mscs;
@@ -77,42 +282,6 @@ Definition atomic_cp_recover T rx : prog T :=
   rx ^(mscs, fsxp).
 
 
-(* XXX need to prove this one ...*)
-Lemma dirtree_update_add_dents: forall name elem' elem dents,
-       map (DIRTREE.update_subtree_helper (fun _ : DIRTREE.dirtree => elem') name)
-           (DIRTREE.add_to_list name elem dents) = DIRTREE.add_to_list name elem' dents.
-Proof.
-      intros.
-Admitted.
-
-
-(* XXX need to prove this one ...*)
-Lemma dirtree_delete_add_dents: forall temp_fn elem tree_elem,
-  DIRTREE.delete_from_list temp_fn (DIRTREE.add_to_list temp_fn elem tree_elem)
-  = tree_elem.
-Proof.
-  intros.
-Admitted.
-
-(* XXX need to prove this one ...*)
-Lemma dirtree_find_add_dents: forall temp_fn elem tree_elem,
-  DIRTREE.find_dirlist temp_fn (DIRTREE.add_to_list temp_fn elem tree_elem)
-  = Some elem.
-Proof.
-  intros.
-Admitted.
-
-(* XXX need to prove this one ...*)
-Lemma dirtree_prune_upd: forall dnum tree_elem dents temp_fn elem elem',
-    dents = map (DIRTREE.update_subtree_helper
-                   (fun _ : DIRTREE.dirtree => elem') temp_fn)
-                   (DIRTREE.add_to_list temp_fn elem tree_elem)
-    ->  (DIRTREE.tree_prune the_dnum dents [] temp_fn
-                            (DIRTREE.TreeDir dnum dents))
-        = (DIRTREE.TreeDir dnum tree_elem).
-Proof.
-    intros.
-Admitted.
 
 Theorem atomic_cp_ok : forall fsxp src_fn dst_fn mscs,
   {< m Fm Ftop tree tree_elem,
@@ -149,112 +318,119 @@ Proof.
   (* [src_fn] points to a file.  destruct [x], consider both cases, one will be false. *)
   destruct x; try solve [ exfalso; eauto ].
 
-  step.
-  instantiate (pathname0 := [] ++ [src_fn]).
-  rewrite DIRTREE.find_subtree_tree_graft_ne by auto.
-  simpl.
-  rewrite H3.
- reflexivity.
-
-  step.
-  instantiate (pathname0 := [] ++ [src_fn]).
-  rewrite DIRTREE.find_subtree_tree_graft_ne by auto.
+  step.  (* file_copy *)
+  
+  rewrite dirtree_add_dents_ne by auto.
   simpl.
   rewrite H3.
   reflexivity.
 
-  (* Here [step] instantiates things incorrectly, so need to do this manually.. *)
-  eapply pimpl_ok2. eauto with prog. cancel.
+  rewrite dirtree_find_add_dents'.
+  eauto.
+  eauto.
 
-  instantiate (pathname0 := [] ++ [temp_fn]).
-  rewrite DIRTREE.find_subtree_tree_graft by auto.
-  reflexivity.
+  step. (* rename *)
+  
+  instantiate (cwd := []).
+  simpl. subst. eauto.
+  
+  step. (* return *)
 
-  instantiate (Fi := emp). constructor.
-
-  simpl; omega.
-
-  step.
-  instantiate (cwd := []). simpl. subst. eauto.
-
-  step.
   eapply pimpl_or_r. right.
   eapply pimpl_or_r. right.
   cancel.
+  
+
+  instantiate (old_inum := w0).
+  instantiate (bytes0 := l).
+  instantiate (attr0 := b1).
   eauto.
 
   (* we got rid of the temporary file in the tree *)
-
   rewrite dirtree_update_add_dents.
-  remember ((DIRTREE.add_to_list temp_fn
-                                 (DIRTREE.TreeFile inum bytes' BYTEFILE.attr0) tree_elem))
-    as dents'.
-  rewrite dirtree_prune_upd with (elem' :=  DIRTREE.TreeFile inum bytes' BYTEFILE.attr0) (elem := DIRTREE.TreeFile inum [] BYTEFILE.attr0) (tree_elem := tree_elem).
-
-  (* src file == dst file *)
-  
-  assert (subtree =  (DIRTREE.TreeFile inum bytes' BYTEFILE.attr0)).
-  rewrite dirtree_update_add_dents in H26.
-  rewrite dirtree_find_add_dents in H26.
-  inversion H26; eauto.
-  rewrite H0.
-
+  rewrite dirtree_prune_add_dents with (elem := (DIRTREE.TreeFile inum l b1)) (tree_elem := tree_elem).
+  rewrite dirtree_update_add_dents in H21.
+  rewrite dirtree_find_add_dents in H21.
   instantiate (new_inum := inum).
-
-  eapply star_emp_pimpl in H20.
-  apply list2nmem_array_eq in H20.
-  rewrite Nat.min_r in H15.
-  apply arrayN_list2nmem in H11.
-  assert (skipn 0 l = l).
-  admit.  (* there must be a lemma for this ...*)
-  rewrite H10 in H11.
-  rewrite Array.firstn_oob in H11.
-  rewrite <- H11.
-  rewrite <- H20.
+  inversion H21.
+  rewrite dirtree_update_add_dents in H20.
+  rewrite dirtree_prune_add_dents with (elem :=  (DIRTREE.TreeFile inum l b1)) (tree_elem := tree_elem) in H20.
+  inversion H20.
+  reflexivity.
+  reflexivity.
+  reflexivity.
   
-  admit. (* XXX b1 = BYTEFILE.attr0; we need to set attr for new file! *)
-  admit.
-  omega.
-
-  assumption.
-    
+  rewrite dirtree_update_add_dents.
   instantiate (pathname1 := []).
-  simpl. reflexivity.
-
+  instantiate (tree_elem0 :=  (DIRTREE.add_to_list temp_fn (DIRTREE.TreeFile inum l b1) tree_elem)).
+  subst; simpl; eauto.
+  
   step.
+
   eapply pimpl_or_r. right.
   eapply pimpl_or_r. left.
   cancel.
 
-  unfold DIRTREE.tree_graft.
-  unfold DIRTREE.add_to_dir.
-  subst; simpl.
-
-  (* two ways of adding the temp file name are the same *)
-  rewrite dirtree_update_add_dents. 
-  instantiate (tbytes := bytes').   
-  instantiate (inum0 := inum).
-  instantiate (tattr := BYTEFILE.attr0).  (* XXX need update when set attr *)
+  rewrite dirtree_update_add_dents.
+  rewrite dirtree_graft_add_dents_eq; auto.
+    
+  eapply pimpl_or_r. left.
+  cancel.
+  rewrite dirtree_delete_add_dents.
   reflexivity.
 
+  pimpl_crash. cancel. apply pimpl_any.
+  pimpl_crash. cancel. apply pimpl_any.
+
+  instantiate (pathname := []).
+  instantiate (tree_elem1 := (DIRTREE.add_to_list temp_fn
+             (DIRTREE.TreeFile inum [] BYTEFILE.attr0) tree_elem)).
+  unfold DIRTREE.find_subtree; subst; simpl.
+  reflexivity.
+
+  step.
+
+  eapply pimpl_or_r. left.
+  cancel.
+  rewrite dirtree_delete_add_dents.
+  reflexivity.
+
+  pimpl_crash. cancel. apply pimpl_any.
+
+  rewrite dirtree_update_add_dents in H16.
+  instantiate (tree_elem2 := (DIRTREE.add_to_list temp_fn (DIRTREE.TreeFile inum bytes' attr')
+             tree_elem)).
+  instantiate (pathname0 := []).
+  rewrite H16.
+  unfold DIRTREE.find_subtree; subst; simpl.
+  reflexivity.
+  
+  step.
+
+  eapply pimpl_or_r. right.
   eapply pimpl_or_r. left.
   cancel.
 
   rewrite dirtree_update_add_dents.
-  rewrite dirtree_delete_add_dents.
-  reflexivity.
-    
-  all: try apply pimpl_any.
-  instantiate (pathname0 := []). simpl.
-  unfold DIRTREE.tree_graft. simpl. reflexivity.
+  rewrite dirtree_graft_add_dents_eq; auto.
+  unfold DIRTREE.tree_graft.
+  unfold DIRTREE.add_to_dir.
+  unfold DIRTREE.update_subtree.
+  eauto.
 
-  step.
   eapply pimpl_or_r. left.
   cancel.
   rewrite dirtree_delete_add_dents.
   reflexivity.
+  
+  pimpl_crash. cancel. apply pimpl_any.
+  pimpl_crash. cancel. apply pimpl_any.
+  pimpl_crash. cancel. apply pimpl_any.
 
-    subst. pimpl_crash. cancel. apply pimpl_any.
-Admitted.
+  Grab Existential Variables.
+  all: eauto.
+Qed.
+
+
 
 
